theories/L6_PCPS/Heap/heap_impl.v
@@ -1,9 +1,9 @@
 From Coq Require Import NArith.BinNat Relations.Relations MSets.MSets
          MSets.MSetRBT Lists.List omega.Omega Sets.Ensembles Relations.Relations
          Classes.Morphisms Sorting.Permutation.
-From ExtLib Require Import Structures.Monad Data.Monads.OptionMonad Core.Type.
-From CertiCoq.L6 Require Import Ensembles_util functions List_util cps set_util Heap.heap.
-Require Import compcert.lib.Coqlib.
+From CertiCoq.L6 Require Import Ensembles_util functions List_util cps set_util.
+From CertiCoq.L6.Heap Require Import heap.
+From compcert.lib Require Import Coqlib.
 
 Import ListNotations.
 
